Changes forgotten by God and the people. New scripts for (re)building and cleaning the project. Implemented heapsort based on leftist heaps and proved it correct (although it's very slow, because it constantly recomputes the legth of the right spine).

Trees/BST.v
@@ -2,7 +2,7 @@ Add Rec LoadPath "/home/zeimer/Code/Coq".
 
 Require Import BTree.
 Require Export LinDec.
-Require Import Sort.
+Require Import Sorting.Sort.
 
 From mathcomp Require Import ssreflect.
 
@@ -160,24 +160,6 @@ Proof.
         apply H7. assumption.
 Qed.
 
-Fixpoint toList {A : LinDec} (t : BTree A) : list A :=
-match t with
-    | empty => []
-    | node v l r => toList l ++ v :: toList r
-end.
-
-Lemma elem_In :
-  forall (A : LinDec) (x : A) (t : BTree A),
-    In x (toList t) <-> elem x t.
-Proof.
-  split.
-    elim: t x => [| v l Hl r Hr] x H.
-      inversion H.
-      cbn in H. apply in_app_or in H. do 2 (destruct H; subst; auto).
-    elim: t x => [| v l Hl r Hr] x H //=; inversion H; subst;
-    apply in_or_app; cbn; eauto.
-Qed.
-
 Theorem toList_sorted : forall (A : LinDec) (t : BTree A),
     is_bst t -> sorted A (toList t).
 Proof.
@@ -191,7 +173,7 @@ Proof.
           rewrite <- H0. auto.
 Qed.
 
-Fixpoint fromList (A : LinDec) (l : list A) : BTree A :=
+Function fromList (A : LinDec) (l : list A) : BTree A :=
 match l with
     | [] => empty
     | h :: t => BTree_ins h (fromList A t)
@@ -199,13 +181,6 @@ end.
 
 Definition treeSort (A : LinDec) (l : list A) : list A :=
     toList (fromList A l).
-
-Functional Scheme fromList_ind := Induction for fromList Sort Prop.
-
-Compute testl.
-Compute treeSort natle testl.
-
-Check testl.
 
 Fixpoint count_BTree (A : LinDec) (x : A) (t : BTree A) : nat :=
 match t with
