Sorting/QuickSort.v
@@ -3,7 +3,7 @@ Add Rec LoadPath "/home/zeimer/Code/Coq".
 Require Export Coq.Program.Wf.
 Require Export Recdef.
 
-Require Export Sort.
+Require Export Sorting.Sort.
 Require Export ListLemmas.
 
 Require Import InsertionSort.
