Sorting/Test.v
@@ -4,6 +4,8 @@ Require Import InsertionSort.
 Require Import SelectionSort.
 Require Import QuickSort.
 Require Import MergeSort.
+Require Import Heap.
+
 Require Import BST.
 
 Set Implicit Arguments.
@@ -14,16 +16,48 @@ match n with
     | S n' => l ++ cycle n' l
 end.
 
-Time Compute treeSort natle (cycle 1000 testl).
-Time Compute hqs 1024 natle (cycle 1000 testl).
-Time Compute hms 1024 natle (cycle 1000 testl).
+Require Import Coq.Sorting.Heap.
+
+Lemma my_le_trans :
+  forall a b c : nat, a <= b -> b <= c -> a <= c.
+Proof.
+  induction a as [| a']; simpl; intros.
+    omega.
+    omega.
+Defined.
+
+(* Definition hps (l : list nat) : list nat :=
+  proj1_sig (sig_of_sig2
+    (treesort nat le eq le_ge_dec Nat.eq_dec le_trans l)).
+
+Compute hps [].
+
+
+Definition heapsort (A : LinDec) (l : list A) : list A :=
+  proj1_sig (sig_of_sig2
+    (treesort A leq eq (LinDec_leq_dec A) (@LinDec_eq_dec A) leq_trans l)). *)
+
 
 (*Time Compute hms2 128 natle (cycle 100 testl).
 Time Compute ms natle (cycle 100 testl).
 Time Compute ms2 natle (cycle 100 testl).
-Time Compute hms 128 natle (cycle 100 testl).
+Time Compute hms 128 natle (cycle 100 testl). *)
 
-Time Compute qs natle (cycle 500 testl).
-Time Compute insertionSort natle (cycle 500 testl).
-Time Compute ssFun natle (cycle 200 testl).
-Time Compute qs2 natle (cycle 200 testl).*)
+Time Compute qs natle (cycle 50 testl).
+Time Compute insertionSort natle (cycle 50 testl).
+Time Compute ss natle (cycle 50 testl).
+Time Compute qs2 natle (cycle 50 testl).
+
+Time Compute leftistHeapsort natle (cycle 50 testl).
+
+Time Compute hqs 1024 natle (cycle 100 testl).
+Time Compute hms 1024 natle (cycle 100 testl).
+Time Compute treeSort natle (cycle 100 testl).
+Time Compute leftistHeapsort natle (cycle 20 testl).
+
+Time Compute hqs 1024 natle (cycle 2000 [1]).
+Time Compute hms 1024 natle (cycle 2000 [1]).
+Time Compute treeSort natle (cycle 2000 [1]).
+
+(* Slow. Change the implemenation to store the right spine. *)
+Time Compute @leftistHeapsort natle (cycle 300 [1]).
