Trees/Heap.v
@@ -1,0 +1,435 @@
+Add Rec LoadPath "/home/zeimer/Code/Coq".
+
+Require Import BTree.
+Require Export LinDec.
+Require Import Sorting.Sort.
+
+Require Import BST.
+
+Set Implicit Arguments.
+
+Inductive is_heap {A : LinDec} : BTree A -> Prop :=
+    | is_heap_empty : is_heap empty
+    | is_heap_node :
+        forall (v : A) (l r : BTree A),
+          (forall x : A, elem x l -> v ≤ x) -> is_heap l ->
+          (forall x : A, elem x r -> v ≤ x) -> is_heap r ->
+            is_heap (node v l r).
+
+Lemma is_heap_inv_l :
+  forall (A : LinDec) (v : A) (l r : BTree A),
+    is_heap (node v l r) -> is_heap l.
+Proof.
+  inversion 1; eauto.
+Qed.
+
+Lemma is_heap_inv_r :
+  forall (A : LinDec) (v : A) (l r : BTree A),
+    is_heap (node v l r) -> is_heap r.
+Proof.
+  inversion 1; eauto.
+Qed.
+
+Lemma is_heap_inv_leq :
+  forall (A : LinDec) (v : A) (l r : BTree A),
+    is_heap (node v l r) -> forall x : A,
+      elem x (node v l r) -> v ≤ x.
+Proof.
+  do 2 inversion 1; subst; auto.
+Qed.
+
+Hint Resolve is_heap_inv_l is_heap_inv_r.
+
+Fixpoint right_spine {A : Type} (t : BTree A) : nat :=
+match t with
+    | empty => 0
+    | node _ _ r => S (right_spine r)
+end.
+
+Inductive left_biased {A : LinDec} : BTree A -> Prop :=
+    | left_biased_empty : left_biased empty
+    | left_biased_node :
+        forall (v : A) (l r : BTree A),
+          right_spine r <= right_spine l ->
+          left_biased l -> left_biased r ->
+            left_biased (node v l r).
+
+Hint Constructors BTree elem is_heap left_biased.
+
+Record LeftistHeap (A : LinDec) : Type :=
+{
+    tree :> BTree A;
+    tree_is_heap : is_heap tree;
+    tree_is_left_biased : left_biased tree
+}.
+
+Ltac lh x :=
+  let t := fresh "t" in
+  let H := fresh "H" in
+  let H' := fresh "H" in
+    destruct x as [t H H']; destruct t;
+    try inversion H; try inversion H'; subst; cbn.
+
+Ltac inv x := inversion x; subst; auto.
+
+Definition getMin {A : LinDec} (h : LeftistHeap A)
+  : option A := root h.
+
+Theorem getMin_spec :
+  forall (A : LinDec) (h : LeftistHeap A) (m : A),
+    getMin h = Some m -> forall x : A, elem x h -> m ≤ x.
+Proof.
+  lh h; inversion 1; subst. inversion 1; auto.
+Qed.
+
+Definition emptyHeap {A : LinDec} : LeftistHeap A.
+Proof.
+  split with (tree := empty); auto.
+Defined.
+
+Theorem emptyHeap_spec :
+  forall (A : LinDec) (x : A), ~ elem x emptyHeap.
+Proof.
+  inversion 1.
+Qed.
+
+Definition singleton {A : LinDec} (x : A) : LeftistHeap A.
+Proof.
+  split with (tree := node x empty empty);
+  constructor; auto; inversion 1.
+Defined.
+
+Theorem singleton_spec :
+  forall (A : LinDec) (x : A),
+    elem x (singleton x).
+Proof.
+  cbn. constructor.
+Qed.
+
+Theorem singleton_spec' :
+  forall (A : LinDec) (x y : A),
+    x <> y -> ~ elem x (singleton y).
+Proof.
+  inversion 2; subst; try contradiction; inv H2.
+Qed.
+
+Definition balance {A : Type} (v : A) (l r : BTree A) : BTree A :=
+  if right_spine r <=? right_spine l
+  then node v l r
+  else node v r l.
+
+Ltac balance := unfold balance in *;
+match goal with
+    | H : context [right_spine ?r <=? right_spine ?l] |- _ =>
+        destruct (@leqb_spec natle (right_spine r) (right_spine l))
+    | |- context [right_spine ?r <=? right_spine ?l] =>
+        destruct (@leqb_spec natle (right_spine r) (right_spine l))
+end.
+
+Lemma balance_len :
+  forall (A : Type) (v : A) (l r : BTree A),
+    len (balance v l r) = len (node v l r).
+Proof.
+  intros. balance.
+    trivial.
+    apply len_swap.
+Qed.
+
+Lemma balance_elem :
+  forall (A : Type) (x v : A) (l r : BTree A),
+    elem x (balance v l r) <-> elem x (node v l r).
+Proof.
+  intros. balance.
+    firstorder.
+    split; inversion 1; subst; auto.
+Qed.
+
+Require Import Recdef.
+
+Definition sum_of_sizes {A : Type} (p : BTree A * BTree A) : nat :=
+  len (fst p) + len (snd p).
+
+Function merge' {A : LinDec} (p : BTree A * BTree A)
+  {measure sum_of_sizes p} : BTree A :=
+match p with
+    | (empty, t2) => t2
+    | (t1, empty) => t1
+    | (node v l r as t1, node v' l' r' as t2) =>
+        if v <=? v'
+        then balance v l (merge' (r, t2))
+        else balance v' l' (merge' (t1, r'))
+end.
+Proof.
+  1-2: intros; cbn; omega.
+Defined.
+
+Arguments merge' [x] _.
+
+Lemma elem_merge' :
+  forall (A : LinDec) (x : A) (t1 t2 : BTree A),
+    elem x (merge' (t1, t2)) -> elem x t1 \/ elem x t2.
+Proof.
+  intros. remember (t1, t2) as p.
+  functional induction @merge' A p; inv Heqp; clear Heqp; auto.
+    rewrite balance_elem in H. inv H. edestruct IHb; eauto.
+    rewrite balance_elem in H. inv H. edestruct IHb; eauto.
+Qed.
+
+Lemma elem_merge'_v2 :
+  forall (A : LinDec) (x : A) (t1 t2 : BTree A),
+    elem x t1 \/ elem x t2 -> elem x (merge' (t1, t2)).
+Proof.
+  intros. remember (t1, t2) as p.
+  functional induction @merge' A p; inv Heqp; clear Heqp; auto.
+    inv H; inv H0.
+    inv H. inv H0.
+    inv H.
+      rewrite balance_elem. inv H0. apply elem_right.
+        eapply IHb. left. exact H2. reflexivity.
+      rewrite balance_elem. apply elem_right.
+        eapply IHb. right. exact H0. reflexivity.
+    inv H.
+      rewrite balance_elem. apply elem_right.
+        eapply IHb. left. exact H0. reflexivity.
+      rewrite balance_elem. inv H0. apply elem_right.
+        eapply IHb. right. exact H2. reflexivity.
+Qed.
+
+Arguments elem_merge' [A x t1 t2] _.
+
+Theorem merge'_len :
+  forall (A : LinDec) (t1 t2 : BTree A),
+    len (merge' (t1, t2)) = len t1 + len t2.
+Proof.
+  intros. remember (t1, t2) as p.
+  functional induction @merge' A p; inv Heqp; clear Heqp.
+    rewrite balance_len. cbn. rewrite (IHb r (node v' l' r') eq_refl).
+      cbn. omega.
+    rewrite balance_len. cbn. rewrite (IHb (node v l r) r' eq_refl).
+      cbn. omega.
+Qed.
+
+Theorem merge'_is_heap :
+  forall (A : LinDec) (t1 t2 : BTree A),
+    is_heap t1 -> is_heap t2 -> is_heap (merge' (t1, t2)).
+Proof.
+  intros. remember (t1, t2) as p.
+  functional induction @merge' A p; inv Heqp; clear Heqp;
+  inv H; inv H0; balance.
+    constructor; auto.
+      intros. destruct (elem_merge' H1); auto.
+        destruct (leqb_spec v v'); inv e0. eapply leq_trans with v'.
+          apply l1.
+          inv H2.
+      apply (IHb _ _ H7 H0 eq_refl).
+    constructor; auto.
+      intros. destruct (elem_merge' H1); auto.
+        destruct (leqb_spec v v'); inv e0. eapply leq_trans with v'.
+          dec.
+          inv H2.
+      apply (IHb _ _ H7 H0 eq_refl).
+      constructor; auto.
+        intros. destruct (elem_merge' H1); auto.
+          destruct (leqb_spec v v'); inv e0. eapply leq_trans with v.
+            dec.
+            inv H2.
+      apply (IHb _ _ H H11 eq_refl).
+      constructor; auto.
+        intros. destruct (elem_merge' H1); auto.
+          destruct (leqb_spec v v'); inv e0. eapply leq_trans with v.
+            dec.
+            inv H2.
+      apply (IHb _ _ H H11 eq_refl).
+Qed.
+
+Theorem merge'_left_biased :
+  forall (A : LinDec) (t1 t2 : BTree A),
+    left_biased t1 -> left_biased t2 -> left_biased (merge' (t1, t2)).
+Proof.
+  intros. remember (t1, t2) as p.
+  functional induction @merge' A p; inv Heqp; clear Heqp;
+  inv H; inv H0; balance; cbn in *;
+  constructor; auto; try omega.
+    1-2: apply (IHb _ _ H6 H0 eq_refl).
+    1-2: apply (IHb _ _ H H9 eq_refl).
+Qed.
+
+Definition merge {A : LinDec} (h1 h2 : LeftistHeap A)
+  : LeftistHeap A.
+Proof.
+  destruct h1 as [t1 H11 H12], h2 as [t2 H21 H22].
+  split with (tree := @merge' A (t1, t2)).
+  apply merge'_is_heap; assumption.
+  apply merge'_left_biased; assumption.
+Defined.
+
+Definition insert' {A : LinDec} (x : A) (t : BTree A) : BTree A :=
+  merge' (node x empty empty, t).
+
+Definition insert {A : LinDec} (x : A) (h : LeftistHeap A)
+  : LeftistHeap A.
+Proof.
+  split with (tree := merge (singleton x) h).
+    destruct (merge _ _). cbn. assumption.
+    destruct (merge _ _). cbn. assumption.
+Defined.
+
+Theorem insert_spec :
+  forall (A : LinDec) (x y : A) (h : LeftistHeap A),
+    elem x (insert y h) <-> x = y \/ elem x h.
+Proof.
+  split; destruct h; subst; cbn; intros.
+    destruct (elem_merge' H); auto. inv H0; inv H2.
+    destruct H; subst; apply elem_merge'_v2; auto.
+Qed.
+
+Definition deleteMin {A : LinDec} (t : BTree A)
+  : option A * BTree A :=
+match t with
+    | empty => (None, empty)
+    | node v l r => (Some v, merge' (l, r))
+end.
+
+Theorem deleteMin_is_heap :
+  forall (A : LinDec) (m : A) (t t' : BTree A),
+    is_heap t -> deleteMin t = (Some m, t') ->
+      is_heap t'.
+Proof.
+  destruct t; cbn; inversion 1; inversion 1; subst.
+  apply merge'_is_heap; assumption.
+Qed.
+
+Theorem deleteMin_spec :
+  forall (A : LinDec) (m : A) (t t' : BTree A),
+    is_heap t -> deleteMin t = (Some m, t') ->
+      forall x : A, elem x t' -> m ≤ x.
+Proof.
+  destruct t; cbn; inversion 1; inversion 1; subst; cbn.
+  intros. destruct (elem_merge' H0); auto.
+Qed.
+
+Theorem deleteMin_len :
+  forall (A : LinDec) (m : A) (t t' : BTree A),
+    deleteMin t = (Some m, t') -> len t = S (len t').
+Proof.
+  destruct t; cbn; inversion 1; subst. rewrite merge'_len. trivial.
+Qed.
+
+Theorem deleteMin_elem :
+  forall (A : LinDec) (m : A) (t t' : BTree A),
+    deleteMin t = (Some m, t') -> elem m t.
+Proof.
+  destruct t; cbn; inversion 1. constructor.
+Qed.
+
+(* Leftist heapsort *)
+Function fromList {A : LinDec} (l : list A) : BTree A :=
+match l with
+    | [] => emptyHeap
+    | h :: t => insert' h (fromList t)
+end.
+
+Function toList {A : LinDec} (t : BTree A)
+  {measure len t} : list A :=
+match deleteMin t with
+    | (None, _) => []
+    | (Some m, t') => m :: toList t'
+end.
+Proof.
+  destruct t; cbn; inversion 1; inversion 1; subst.
+  rewrite merge'_len. omega.
+Defined.
+
+Arguments toList [x] _.
+
+Definition leftistHeapsort (A : LinDec) (l : list A)
+  : list A := toList (fromList l).
+
+Lemma toList_sorted :
+  forall (A : LinDec) (t : BTree A),
+    is_heap t -> sorted A (toList t).
+Proof.
+  intros A t. functional induction @toList A t.
+    constructor.
+    functional induction @toList A t'; constructor.
+      eapply deleteMin_spec; eauto. eapply deleteMin_elem. eauto.
+      apply IHl. eapply deleteMin_is_heap; eauto.
+Qed.
+
+Lemma fromList_is_heap :
+  forall (A : LinDec) (l : list A),
+    is_heap (fromList l).
+Proof.
+  intros. functional induction @fromList A l; cbn.
+    constructor.
+    unfold insert'. apply merge'_is_heap; auto.
+      constructor; auto; inversion 1.
+Qed.
+
+Theorem leftistHeapsort_sorted :
+  forall (A : LinDec) (l : list A),
+    sorted A (leftistHeapsort A l).
+Proof.
+  unfold leftistHeapsort. intros.
+    apply toList_sorted. apply fromList_is_heap.
+Qed.
+
+Lemma count_BTree_merge' :
+  forall (A : LinDec) (x : A) (t1 t2 : BTree A),
+    count_BTree A x (merge' (t1, t2)) =
+    count_BTree A x t1 + count_BTree A x t2.
+Proof.
+  intros. remember (t1, t2) as p.
+  functional induction @merge' A p; inv Heqp; clear Heqp.
+    balance; cbn.
+      rewrite (IHb _ _ _ eq_refl). dec.
+      rewrite (IHb _ _ _ eq_refl). dec.
+    balance; cbn.
+      rewrite (IHb _ _ _ eq_refl). dec.
+      rewrite (IHb _ _ _ eq_refl). dec.
+Qed.
+
+Lemma count_BTree_insert :
+  forall (A : LinDec) (x y : A) (t : BTree A),
+    count_BTree A x (insert' y t) =
+      if x =? y
+      then S (count_BTree A x t)
+      else count_BTree A x t.
+Proof.
+  intros. unfold insert'. rewrite count_BTree_merge'. dec.
+Qed.
+
+Lemma count_fromList :
+  forall (A : LinDec) (x : A) (l : list A),
+    count_BTree A x (fromList l) = count A x l.
+Proof.
+  intros. functional induction @fromList A l; dec.
+    rewrite count_BTree_insert. dec.
+    rewrite count_BTree_insert. dec.
+Qed.
+
+Lemma count_toList :
+  forall (A : LinDec) (x : A) (t : BTree A),
+    count A x (toList t) = count_BTree A x t.
+Proof.
+  intros. functional induction @toList A t; cbn.
+    destruct t; inv e.
+    destruct t; inv e. dec.
+      rewrite IHl, count_BTree_merge'. trivial.
+      rewrite IHl, count_BTree_merge'. trivial.
+Qed.
+
+Theorem leftistHeapsort_perm :
+  forall (A : LinDec) (l : list A),
+    perm A l (leftistHeapsort A l).
+Proof.
+  unfold perm, leftistHeapsort. intros.
+  rewrite count_toList, count_fromList. trivial.
+Qed.
+
+Instance Sort_leftistHeapsort : Sort :=
+{
+    sort := @leftistHeapsort;
+    sort_sorted := @leftistHeapsort_sorted;
+    sort_perm := leftistHeapsort_perm
+}.
