new_rebuild.sh
@@ -1,0 +1,4 @@
+#!/bin/bash
+./clean.sh
+./make_makefile.sh
+make
